It can be shown that:
$$ax^{2} + bx + c = a\left( x+\frac{b^{2}}{2a} \right)^{2}+\left( c-\frac{b^{2}}{4a^{2}} \right)$$
## Example 1
*Write $3x^{2}+6x+1$ in the form $p(x+q)^{2} + r$*
### Method 1
$$
\begin{gather*}
3x^{3}+6x+1 \\ \\
= 3\left( x^{2}+\frac{6^{2}}{2(3)} \right)^{2}+\left( 1-\frac{6^{2}}{4(3)^{2}} \right) \\ \\
= 3(x+1)^{2} - 2
\end{gather*}

$$
### Method 2
$$
\begin{gather*}
3x^{2} + 6x+1 \\
= 3(x^{2}+2x) + 1 \\
= 3((x+1)^{2}-1) + 1 \\
= 3(x+1)^{2} - 3 + 1 \\
= 3(x+1)^{2} - 2
\end{gather*}
$$