It is possible to show that:
$$
\sqrt{\sum_{r=1}^nr^{3}} = \sum_{r=1}^nr
$$
and:
$$
\left( \sum_{r=1}^nr \right)^{2}=\sum_{r=1}^nr^{3}
$$
This is because:
$$
\left( \frac{n(n+1)}{2} \right)^{2}=\frac{1}{4}n^{2}(n+1)^{2}
$$
This is useful for in an example like this:
*E.g. Compute $\sum_{r=1}^3r_{3}$*
$$
\begin{gather*}
\sum_{r=1}^3r = 1 + 2 + 3 = 6 \\ \\
\therefore \sum_{r=1}^3r_{3} = (\sum_{r=1}^3r )^{2} = 6^{2} = 36
\end{gather*}
$$
Another example:
*Compute $\sum_{r=1}^{10}r^{3}$*
$$
\sum_{r=1}^{10}r^{3} = \left(\frac{10(11)}{2}\right)^{2} = 55^{2} = 3025
$$
This might faster than typing $\frac{1}{4}(10)^{2}(11)^{2}$ into your calculator 

## Problem solving example:
*Find n such that $\sum_{r=1}^nr^{3}=8281$*

In this scenario, it might be easier to use $\left(\frac{n(n+1)}{2}\right)^{2}$ than $\frac{1}{4}n^{2}(n+1)^{2}$

$$

$$